specs/lemmas/Spec.SHA2.Lemmas.fsti
@@ -9,8 +9,8 @@ val update_224_256: hash:words_state SHA2_256 ->
   Lemma
     (ensures (Spec.SHA2.(update SHA2_256 hash block == update SHA2_224 hash block)))
 
-val update_multi_224_256: hash:words_state SHA2_256 -> prev:nat -> blocks:bytes_blocks SHA2_256 ->
+val update_multi_224_256: hash:words_state SHA2_256 -> blocks:bytes_blocks SHA2_256 ->
   Lemma
-    (ensures (Spec.Agile.Hash.update_multi SHA2_256 hash prev blocks ==
-      Spec.Agile.Hash.update_multi SHA2_224 hash prev blocks))
+    (ensures (Spec.Agile.Hash.update_multi SHA2_256 hash () blocks ==
+      Spec.Agile.Hash.update_multi SHA2_224 hash () blocks))
     (decreases (Seq.length blocks))
